specIR/SIRmini.v
@@ -1,0 +1,335 @@
+From Coq Require Import
+     Arith.PeanoNat
+     Lists.List
+     Strings.String
+     Morphisms
+     Setoid
+     RelationClasses.
+
+Require Import MapsC.
+Require Import ValuesC.
+Require Import MemoryC.
+Require Import CoqlibC.
+Require Import ASTC.
+Require Import EventsC.
+Require Import GlobalenvsC.
+Require Import IntegersC.
+Require Import Mod ModSem Any Skeleton.
+Require Export SIRCommon.
+
+Require Import Program.
+Require Import Simulation.
+
+Set Implicit Arguments.
+
+
+
+
+
+Section OWNEDHEAP.
+
+Variable owned_heap: Type.
+
+
+
+
+
+Section EFF.
+
+  Variant InternalCallE: Type -> Type :=
+  | ICall (name: ident) (oh: owned_heap) (m: mem) (vs: list val):
+      InternalCallE (owned_heap * (mem * val))
+  .
+
+  Variant EventE: Type -> Type :=
+  | ENB: EventE void
+  | EUB: EventE void
+  | ESyscall (ef: external_function) (m: mem) (args: list val): EventE (val * mem)
+  | ECall (fptr: val) (oh: owned_heap) (m: mem) (vs: list val): EventE (owned_heap * (mem * val))
+  .
+
+  Variant DoneE: Type -> Type :=
+  | EDone (oh: owned_heap) (m: mem) (v: val): DoneE void
+  .
+
+  Definition eff0: Type -> Type := Eval compute in ExternalCallE +' DoneE +' EventE.
+  Definition eff1: Type -> Type := Eval compute in InternalCallE +' eff0.
+  Definition E := Eval compute in eff1.
+
+End EFF.
+
+(* Q: Why manually match "void" type, not using "embed" or "trigger"?
+   A: It returns arbitrary type "A", not "void" *)
+Definition triggerUB {E A} `{EventE -< E}: itree E A :=
+  vis (EUB) (fun v => match v: void with end)
+.
+Definition triggerNB {E A} `{EventE -< E}: itree E A :=
+  vis (ENB) (fun v => match v: void with end)
+.
+Definition triggerDone {E A} `{DoneE -< E} (oh: owned_heap) (m: mem) (v: val): itree E A :=
+  vis (EDone oh m v) (fun v => match v: void with end)
+.
+
+Definition unwrapN {E X} `{EventE -< E} (x: option X): itree E X :=
+  match x with
+  | Some x => ret x
+  | None => triggerNB
+  end.
+
+Definition unwrapU {E X} `{EventE -< E} (x: option X): itree E X :=
+  match x with
+  | Some x => ret x
+  | None => triggerUB
+  end.
+
+Record function : Type := mkfunction
+  { fn_sig: signature;
+    fn_code: (forall (oh: owned_heap) (m: mem) (vs: list val),
+                 itree E (owned_heap * (mem * val))); }
+.
+
+Definition program: Type := AST.program (fundef function) unit.
+
+
+
+
+
+Section DENOTE.
+
+  Variable p: program.
+  Variable ge: SkEnv.t.
+
+  Definition interp_function: (InternalCallE ~> itree E) :=
+    fun T ei =>
+      let '(ICall func_name oh m vs) := ei in
+      match (find (fun nf => ident_eq func_name (fst nf)) p.(prog_defs)) with
+      | Some (_, Gfun (Internal f)) =>
+        (f.(fn_code) oh m vs)
+      | _ => triggerNB
+      end
+  .
+
+  Definition interp_program0:
+    (forall T, InternalCallE T -> itree eff0 T) :=
+    fun _ ic =>
+      let sem0: itree eff0 _ := (mrec interp_function) _ ic in
+      sem0
+  .
+
+End DENOTE.
+
+
+
+
+
+
+Section TEST.
+
+Definition _sum := 55%positive.
+  
+Definition c_sum (oh: owned_heap) (m: mem) (vs: list val): itree E (owned_heap * (mem * val)) :=
+  match vs with
+  | [Vint n] =>
+    if Int.eq n Int.zero
+    then Ret (oh, (m, (Vint Int.zero)))
+    else '(oh, (m, s)) <- trigger (ICall _sum oh m [Vint (Int.sub n Int.one)]) ;;
+         Ret (oh, (m, (Val.add s (Vint n))))
+  | _ => triggerUB
+  end
+.
+
+Definition f_sum: function :=
+  mkfunction signature_main c_sum
+.
+
+Definition global_definitions: list (ident * globdef (fundef (function)) unit) :=
+  ((_sum, Gfun(Internal f_sum)) :: nil)
+.
+
+Definition p: program := mkprogram global_definitions nil 1%positive.
+
+Variable initial_oh: owned_heap.
+Let one := (interp_program0 p (ICall _sum initial_oh Mem.empty [Vint (Int.repr 1%Z)])).
+(* Compute (burn 1 one). *)
+
+Lemma one_spec
+  :
+    one ≈ Ret (initial_oh, (Mem.empty, Vint (Int.repr 1%Z)))
+.
+Proof.
+  subst one. unfold interp_program0. ss.
+  rewrite mrec_as_interp. cbn. des_ifs. cbn. des_ifs.
+  autorewrite with itree. cbn.
+  rewrite mrec_as_interp. cbn. des_ifs. cbn. des_ifs.
+  autorewrite with itree. cbn.
+  replace (Int.add Int.zero (Int.repr 1)) with (Int.repr 1); cycle 1.
+  { refl. }
+  refl.
+Qed.
+
+End TEST.
+
+
+
+
+
+Section MODSEM.
+
+  Variable mi: string.
+  Variable skenv_link: SkEnv.t.
+  Variable initial_owned_heap: owned_heap.
+  Variable p: program.
+  Let skenv: SkEnv.t := (SkEnv.project skenv_link) (Sk.of_program fn_sig p).
+  (* Let ge: genv := (SkEnv.revive skenv) p. *)
+  Definition genvtype: Type := unit.
+  Let ge: genvtype := tt.
+
+  Record state := mk {
+    itr:> itree eff0 (owned_heap * (mem * val));
+  }.
+
+  Let interp_program0 := interp_program0 p.
+
+  Inductive initial_frame (oh0: owned_heap) (args: Args.t): state -> Prop :=
+  | initial_frame_intro
+      itr fid blk m0 vs fd tvs
+      (FPTR: (Args.fptr args) = Vptr blk Ptrofs.zero)
+      (VS: (Args.vs args) = vs)
+      (M: (Args.m args) = m0)
+
+      (SYMB: Genv.find_symbol skenv fid = Some blk)
+      (FINDF: Genv.find_funct skenv (Vptr blk Ptrofs.zero) = Some (Internal fd))
+      (TYP: typecheck (Args.vs args) fd tvs)
+
+      st0
+      (ITR: itr = (interp_program0 (ICall fid oh0 m0 vs)))
+      (ST: st0 = (mk itr))
+    :
+      initial_frame oh0 args st0
+  .
+
+  Inductive at_external (st0: state): owned_heap -> Args.t -> Prop :=
+  | at_external_intro
+      args fptr vs k oh0 m0
+      (VIS: st0.(itr) = Vis (subevent _ (ECall fptr oh0 m0 vs)) k)
+      (ARGS: args = Args.mk fptr vs m0)
+    :
+      at_external st0 oh0 args
+  .
+
+  Inductive get_k (st0: state):
+    (owned_heap * (mem * val) -> itree eff0 (owned_heap * (mem * val))) -> Prop :=
+  | get_k_intro
+      _vs _fptr _oh0 _m0 k
+      (VIS: st0.(itr) = Vis (subevent _ (ECall _fptr _oh0 _m0 _vs)) k)
+    :
+      get_k st0 k
+  .
+
+  Inductive after_external (st0: state) (oh0: owned_heap) (retv: Retv.t): state -> Prop :=
+  | after_external_intro
+      k m0 rv st1
+      (GETK: get_k st0 k)
+      (V: (Retv.v retv) = rv)
+      (M: (Retv.m retv) = m0)
+      (KONT: st1 = mk (k (oh0, (m0, rv))))
+    :
+      after_external st0 oh0 retv st1
+  .
+
+  Inductive final_frame (st0: state): owned_heap -> Retv.t -> Prop :=
+  | final_frame_intro
+      oh0 m0 (rv: val) retv
+      (RET: st0.(itr) = Ret (oh0, (m0, rv)))
+      (RETV: retv = Retv.mk rv m0)
+    :
+      final_frame st0 oh0 retv
+  .
+
+  Inductive step (se: Senv.t) (ge: genvtype) (st0: state) (tr: trace) (st1: state): Prop :=
+  (* | step_tau *)
+  (*     itr0 *)
+  (*     itr1 *)
+  (*     (TAU: st0.(itr) = Tau itr1) *)
+
+  (*     (ST0: st0 = mk itr0) *)
+  (*     (TR: tr = E0) *)
+  (*     (ST1: st1 = mk itr1) *)
+  (*** ub is stuck, so we don't state anything ***)
+  | step_nb
+      k
+      (VIS: st0.(itr) = Vis (subevent _ (ENB)) k)
+
+      (TR: tr = E0)
+  | step_syscall
+      itr0 m0 m1
+      ef vs rv k
+      (VIS: st0.(itr) = Vis (subevent _ (ESyscall ef m0 vs)) k)
+      (SYSCALL: external_call ef se vs m0 tr rv m1)
+
+      (ST0: st0 = mk itr0)
+      (TR: tr = E0)
+      (ST1: st1 = mk (k (rv, m1)))
+  | step_done
+      itr0
+      oh rv m k
+      (VIS: st0.(itr) = Vis (subevent _ (EDone oh m rv)) k)
+
+      (ST0: st0 = mk itr0)
+      (TR: tr = E0)
+      (ST1: st1 = mk (Ret (oh, (m, rv))))
+  .
+
+  Program Definition modsem: ModSem.t :=
+    {| ModSem.step := step;
+       ModSem.owned_heap := owned_heap;
+       ModSem.at_external := at_external;
+       ModSem.initial_frame := initial_frame;
+       ModSem.final_frame := final_frame;
+       ModSem.after_external := after_external;
+       ModSem.initial_owned_heap := initial_owned_heap;
+       ModSem.globalenv := ge;
+       ModSem.skenv := skenv;
+       ModSem.skenv_link := skenv_link;
+       ModSem.midx := Some mi;
+    |}.
+  Next Obligation.
+    inv AT0. inv AT1. rewrite VIS in *. des. clarify.
+  Qed.
+  Next Obligation.
+    inv FINAL0. inv FINAL1. rewrite RET in *. des. clarify.
+  Qed.
+  Next Obligation.
+    inv AFTER0. inv AFTER1. inv GETK. inv GETK0. rewrite VIS in *.
+    ss. clarify. simpl_depind. clarify.
+  Qed.
+  Next Obligation.
+    ii. des. inv PR; ss. destruct x0; ss. clarify. inv PR0; ss.
+  Qed.
+  Next Obligation.
+    ii. des. inv PR0; ss. inv PR; ss; clarify; try rewrite RET in *; ss; clarify.
+  Qed.
+  Next Obligation.
+    ii. des. inv PR; ss. inv PR0; ss; clarify; try rewrite VIS in *; ss; clarify.
+  Qed.
+
+  Lemma modsem_receptive: forall st, receptive_at modsem st.
+  Proof.
+    econs; eauto.
+    - ii; ss. inv H; try (exploit external_call_receptive; eauto; check_safe; intro T; des); inv_match_traces; try (by esplits; eauto; econs; eauto).
+    - ii. inv H; try (exploit external_call_trace_length; eauto; check_safe; intro T; des); ss; try xomega.
+  Unshelve.
+    all: ss.
+  Qed.
+
+End MODSEM.
+
+Program Definition module (p: program) (mi: string) (initial_owned_heap: SkEnv.t -> owned_heap): Mod.t :=
+  {| Mod.data := p; Mod.get_sk := (Sk.of_program fn_sig);
+     Mod.get_modsem := fun skenv_link p => modsem mi skenv_link
+                                                  (initial_owned_heap skenv_link) p;
+     Mod.midx := Some mi |}
+.
+
+End OWNEDHEAP.
+
