specIR/SIRmini_eutt.v
@@ -1,0 +1,415 @@
+From Coq Require Import
+     Arith.PeanoNat
+     Lists.List
+     Strings.String
+     Morphisms
+     Setoid
+     RelationClasses.
+
+Require Import MapsC.
+Require Import ValuesC.
+Require Import MemoryC.
+Require Import CoqlibC.
+Require Import ASTC.
+Require Import EventsC.
+Require Import GlobalenvsC.
+Require Import IntegersC.
+Require Import Mod ModSem Any Skeleton.
+Require Export SIRCommon.
+
+Require Import Program.
+Require Import Simulation.
+
+Set Implicit Arguments.
+
+
+
+
+Open Scope itree_scope.
+
+Lemma eq_eutt
+      E R
+      (a b: itree E R)
+      (EQ: a = b)
+  :
+    eutt eq a b
+.
+Proof. i. clarify. refl. Qed.
+
+Lemma vis_not_ret
+      E R (r: R) X (e: E X) k
+      (EUTT: Vis e k ≈ Ret r)
+  :
+    False
+.
+Proof. ii. punfold EUTT. inv EUTT. Qed.
+
+(* Lemma eqit_inv_vis {E R1 R2 RR} b1 b2 {u1 u2} (e1: E u1) (e2: E u2) *)
+(*       (k1: u1 -> itree E R1) (k2: u2 -> itree E R2) : *)
+(*   eqit RR b1 b2 (Vis e1 k1) (Vis e2 k2) -> *)
+(*   u1 = u2 /\ e1 ~= e2 /\ (forall u1 u2 (EQ: u1 ~= u2), eqit RR b1 b2 (k1 u1) (k2 u2)). *)
+(* Proof. *)
+(*   intros. punfold H. repeat red in H. simpl in H. *)
+(*   dependent destruction H. pclearbot. esplits; eauto. *)
+(*   ii. apply JMeq_eq in EQ. clarify. *)
+(* Qed. *)
+
+Fail Lemma empty_nonempty
+      (T: Type)
+      (EQ: void = T)
+      (INHAB: inhabited T)
+  :
+    False
+.
+(* Proof. *)
+(*   inversion INHAB. rewrite <- EQ in H. inv H. *)
+(* Qed. *)
+
+
+
+
+
+
+
+
+Section OWNEDHEAP.
+
+Variable owned_heap: Type.
+
+
+
+
+
+Section EFF.
+
+  Variant InternalCallE: Type -> Type :=
+  | ICall (name: ident) (oh: owned_heap) (m: mem) (vs: list val):
+      InternalCallE (owned_heap * (mem * val))
+  .
+
+  Variant EventE: Type -> Type :=
+  | ENB: EventE void
+  | EUB: EventE void
+  | ESyscall (ef: external_function) (m: mem) (args: list val): EventE (val * mem)
+  | ECall (fptr: val) (oh: owned_heap) (m: mem) (vs: list val): EventE (owned_heap * (mem * val))
+  .
+
+  Variant DoneE: Type -> Type :=
+  | EDone (oh: owned_heap) (m: mem) (v: val): DoneE void
+  .
+
+  Definition eff0: Type -> Type := Eval compute in ExternalCallE +' DoneE +' EventE.
+  Definition eff1: Type -> Type := Eval compute in InternalCallE +' eff0.
+  Definition E := Eval compute in eff1.
+
+End EFF.
+
+(* Q: Why manually match "void" type, not using "embed" or "trigger"?
+   A: It returns arbitrary type "A", not "void" *)
+Definition triggerUB {E A} `{EventE -< E}: itree E A :=
+  vis (EUB) (fun v => match v: void with end)
+.
+Definition triggerNB {E A} `{EventE -< E}: itree E A :=
+  vis (ENB) (fun v => match v: void with end)
+.
+Definition triggerDone {E A} `{DoneE -< E} (oh: owned_heap) (m: mem) (v: val): itree E A :=
+  vis (EDone oh m v) (fun v => match v: void with end)
+.
+
+Definition unwrapN {E X} `{EventE -< E} (x: option X): itree E X :=
+  match x with
+  | Some x => ret x
+  | None => triggerNB
+  end.
+
+Definition unwrapU {E X} `{EventE -< E} (x: option X): itree E X :=
+  match x with
+  | Some x => ret x
+  | None => triggerUB
+  end.
+
+Record function : Type := mkfunction
+  { fn_sig: signature;
+    fn_code: (forall (oh: owned_heap) (m: mem) (vs: list val),
+                 itree E (owned_heap * (mem * val))); }
+.
+
+Definition program: Type := AST.program (fundef function) unit.
+
+
+
+
+
+Section DENOTE.
+
+  Variable p: program.
+  Variable ge: SkEnv.t.
+
+  Definition interp_function: (InternalCallE ~> itree E) :=
+    fun T ei =>
+      let '(ICall func_name oh m vs) := ei in
+      match (find (fun nf => ident_eq func_name (fst nf)) p.(prog_defs)) with
+      | Some (_, Gfun (Internal f)) =>
+        (f.(fn_code) oh m vs)
+      | _ => triggerNB
+      end
+  .
+
+  Definition interp_program0:
+    (forall T, InternalCallE T -> itree eff0 T) :=
+    fun _ ic =>
+      let sem0: itree eff0 _ := (mrec interp_function) _ ic in
+      sem0
+  .
+
+End DENOTE.
+
+
+
+
+
+
+Section TEST.
+
+Definition _sum := 55%positive.
+  
+Definition c_sum (oh: owned_heap) (m: mem) (vs: list val): itree E (owned_heap * (mem * val)) :=
+  match vs with
+  | [Vint n] =>
+    if Int.eq n Int.zero
+    then Ret (oh, (m, (Vint Int.zero)))
+    else '(oh, (m, s)) <- trigger (ICall _sum oh m [Vint (Int.sub n Int.one)]) ;;
+         Ret (oh, (m, (Val.add s (Vint n))))
+  | _ => triggerUB
+  end
+.
+
+Definition f_sum: function :=
+  mkfunction signature_main c_sum
+.
+
+Definition global_definitions: list (ident * globdef (fundef (function)) unit) :=
+  ((_sum, Gfun(Internal f_sum)) :: nil)
+.
+
+Definition p: program := mkprogram global_definitions nil 1%positive.
+
+Variable initial_oh: owned_heap.
+Let one := (interp_program0 p (ICall _sum initial_oh Mem.empty [Vint (Int.repr 1%Z)])).
+(* Compute (burn 1 one). *)
+
+Lemma one_spec
+  :
+    one ≈ Ret (initial_oh, (Mem.empty, Vint (Int.repr 1%Z)))
+.
+Proof.
+  subst one. unfold interp_program0. ss.
+  rewrite mrec_as_interp. cbn. des_ifs. cbn. des_ifs.
+  autorewrite with itree. cbn.
+  rewrite mrec_as_interp. cbn. des_ifs. cbn. des_ifs.
+  autorewrite with itree. cbn.
+  replace (Int.add Int.zero (Int.repr 1)) with (Int.repr 1); cycle 1.
+  { refl. }
+  refl.
+Qed.
+
+End TEST.
+
+
+
+
+
+Section MODSEM.
+
+  Variable mi: string.
+  Variable skenv_link: SkEnv.t.
+  Variable initial_owned_heap: owned_heap.
+  Variable p: program.
+  Let skenv: SkEnv.t := (SkEnv.project skenv_link) (Sk.of_program fn_sig p).
+  (* Let ge: genv := (SkEnv.revive skenv) p. *)
+  Definition genvtype: Type := unit.
+  Let ge: genvtype := tt.
+
+  Inductive state: Type :=
+  | State
+      (itr: itree eff0 (owned_heap * (mem * val)))
+  | Callstate
+      (fptr: val)
+      (oh0: owned_heap)
+      (m0: mem)
+      (vs: list val)
+      (k: (owned_heap * (mem * val)) -> itree eff0 (owned_heap * (mem * val)))
+  .
+
+  (* Record state := mk { *)
+  (*   itr:> itree eff0 (owned_heap * (mem * val)); *)
+  (* }. *)
+
+  Let interp_program0 := interp_program0 p.
+
+  Inductive initial_frame (oh0: owned_heap) (args: Args.t): state -> Prop :=
+  | initial_frame_intro
+      itr fid blk m0 vs fd tvs
+      (FPTR: (Args.fptr args) = Vptr blk Ptrofs.zero)
+      (VS: (Args.vs args) = vs)
+      (M: (Args.m args) = m0)
+
+      (SYMB: Genv.find_symbol skenv fid = Some blk)
+      (FINDF: Genv.find_funct skenv (Vptr blk Ptrofs.zero) = Some (Internal fd))
+      (TYP: typecheck (Args.vs args) fd tvs)
+
+      st0
+      (ITR: itr ≈ (interp_program0 (ICall fid oh0 m0 vs)))
+      (ST: st0 = (State itr))
+    :
+      initial_frame oh0 args st0
+  .
+
+  Inductive at_external: state -> owned_heap -> Args.t -> Prop :=
+  | at_external_intro
+      fptr vs k oh0 m0
+    :
+      at_external (Callstate fptr oh0 m0 vs k) oh0 (Args.mk fptr vs m0)
+  .
+
+  Inductive after_external: state -> owned_heap -> Retv.t -> state -> Prop :=
+  | after_external_intro
+      fptr oh0 m0 vs oh1 m1 rv
+      k itr0
+      (KONT: itr0 = (k (oh1, (m1, rv))))
+    :
+      after_external (Callstate fptr oh0 m0 vs k) oh1 (Retv.mk rv m1) (State itr0)
+  .
+
+  Inductive final_frame: state -> owned_heap -> Retv.t -> Prop :=
+  | final_frame_intro
+      itr0 oh0 m0 (rv: val)
+      (RET: itr0 ≈ Ret (oh0, (m0, rv)))
+    :
+      final_frame (State itr0) oh0 (Retv.mk rv m0)
+  .
+
+  Inductive step (se: Senv.t) (ge: genvtype): state -> trace -> state -> Prop :=
+  (* | step_tau *)
+  (*     itr0 *)
+  (*     itr1 *)
+  (*     (TAU: st0.(itr) = Tau itr1) *)
+
+  (*     (ST0: st0 = mk itr0) *)
+  (*     (TR: tr = E0) *)
+  (*     (ST1: st1 = mk itr1) *)
+  (*** ub is stuck, so we don't state anything ***)
+  | step_nb
+      itr0 k
+      (VIS: itr0 ≈ Vis (subevent _ (ENB)) k)
+    :
+      step se ge (State itr0) E0 (State itr0)
+  | step_extcall
+      itr0 k fptr oh0 m0 vs
+      (VIS: itr0 ≈ Vis (subevent _ (ECall fptr oh0 m0 vs)) k)
+    :
+      step se ge (State itr0) E0 (Callstate fptr oh0 m0 vs k)
+  | step_syscall
+      itr0 tr m0 m1
+      ef vs rv k
+      (VIS: itr0 ≈ Vis (subevent _ (ESyscall ef m0 vs)) k)
+      (SYSCALL: external_call ef se vs m0 tr rv m1)
+    :
+      step se ge (State itr0) E0 (State (k (rv, m1)))
+  | step_done
+      itr0
+      oh rv m k
+      (VIS: itr0 ≈ Vis (subevent _ (EDone oh m rv)) k)
+    :
+      step se ge (State itr0) E0 (State (Ret (oh, (m, rv))))
+  .
+
+  Program Definition modsem: ModSem.t :=
+    {| ModSem.step := step;
+       ModSem.owned_heap := owned_heap;
+       ModSem.at_external := at_external;
+       ModSem.initial_frame := initial_frame;
+       ModSem.final_frame := final_frame;
+       ModSem.after_external := after_external;
+       ModSem.initial_owned_heap := initial_owned_heap;
+       ModSem.globalenv := ge;
+       ModSem.skenv := skenv;
+       ModSem.skenv_link := skenv_link;
+       ModSem.midx := Some mi;
+    |}.
+  Next Obligation.
+    inv AT0. inv AT1. esplits; et.
+  Qed.
+  Next Obligation.
+    inv FINAL0. inv FINAL1. rewrite RET in *. apply eqit_inv_ret in RET0. clarify.
+  Qed.
+  Next Obligation.
+    inv AFTER0. inv AFTER1. f_equal.
+  Qed.
+  Next Obligation.
+    ii. des. inv PR; ss; inv PR0; ss.
+  Qed.
+  Next Obligation.
+    ii. des. inv PR; ss; inv PR0; ss; try rewrite VIS in RET; exploit vis_not_ret; et.
+  Qed.
+  Next Obligation.
+    ii. des. inv PR; ss; inv PR0; ss.
+  Qed.
+
+  Lemma modsem_receptive: forall st, receptive_at modsem st.
+  Proof.
+    econs; eauto.
+    - ii; ss. inv H; try (exploit external_call_receptive; eauto; check_safe; intro T; des); inv_match_traces; try (by esplits; eauto; econs; eauto).
+    - ii. inv H; try (exploit external_call_trace_length; eauto; check_safe; intro T; des); ss; try xomega.
+  Unshelve.
+    all: ss.
+  Qed.
+
+  (* Lemma modsem_determinate: forall st, determinate_at modsem st. *)
+  (* Proof. *)
+  (*   econs; eauto. *)
+  (*   - ii; ss. *)
+  (*     inv H; inv H0; esplits; et; try econs; et; *)
+  (*       try by (rewrite VIS in *; punfold VIS0; inv VIS0; simpl_depind; subst; simpl_depind). *)
+  (*     + rewrite VIS in *. apply eqit_inv_vis in VIS0. des. clarify. *)
+  (*       esplits; et. *)
+  (*     + rewrite VIS in *. punfold VIS0. inv VIS0. simpl_depind. subst. simpl_depind. *)
+  (*     + rewrite VIS in *. punfold VIS0. inv VIS0. simpl_depind. subst. simpl_depind. *)
+  (*     + rewrite VIS in *. punfold VIS0. inv VIS0. simpl_depind. subst. simpl_depind. *)
+  (*     + rewrite VIS in *. punfold VIS0. inv VIS0. simpl_depind. subst. simpl_depind. *)
+  (*       exploit empty_nonempty; try apply VIS0. *)
+  (*       { rewrite VIS0. et. *)
+  (*       unfold eutt in *. *)
+  (*       eapply (@eqit_inv_vis eff0 (owned_heap * (mem * val)) (owned_heap * (mem * val)) *)
+  (*                             eq true true *)
+  (*              ) in VIS0. *)
+  (*       eapply (eqit_inv_vis true true (subevent void ENB)) in VIS0. et. *)
+  (*       Set Printing All. *)
+  (*       unfold eutt in VIS0. *)
+  (*       eapply eqit_inv_vis in VIS0. et. *)
+  (*       punfold VIS0. inv VIS0. simpl_depind. subst. simpl_depind. *)
+  (*       eapply eqit_inv_vis in VIS0. et. *)
+  (*     clarify. *)
+  (*     clarify_meq; try (determ_tac eval_expr_determ; check_safe); *)
+  (*               try (determ_tac eval_lvalue_determ; check_safe); try (determ_tac eval_exprlist_determ; check_safe); *)
+  (*                 try (determ_tac eval_builtin_args_determ; check_safe); try (determ_tac external_call_determ; check_safe); *)
+  (*                   esplits; eauto; try (econs; eauto); ii; eq_closure_tac; clarify_meq. *)
+  (*     + inv H4; inv H16; congruence. *)
+  (*     + determ_tac eval_exprlist_determ. *)
+  (*     + inv H1. inv H8. hexploit (alloc_variables_determ H0 H3). i; des; clarify. determ_tac bind_parameters_determ. *)
+  (*   - ii. inv H; try (exploit external_call_trace_length; eauto; check_safe; intro T; des); ss; try xomega. *)
+  (* Unshelve. *)
+  (*   all: des; ss; try (by exfalso; des; ss). *)
+  (* Qed. *)
+
+End MODSEM.
+
+Program Definition module (p: program) (mi: string) (initial_owned_heap: SkEnv.t -> owned_heap): Mod.t :=
+  {| Mod.data := p; Mod.get_sk := (Sk.of_program fn_sig);
+     Mod.get_modsem := fun skenv_link p => modsem mi skenv_link
+                                                  (initial_owned_heap skenv_link) p;
+     Mod.midx := Some mi |}
+.
+
+End OWNEDHEAP.
+
